specs/ecdsap256sha2/Spec.P256.MontgomeryMultiplication.fsti
@@ -10,12 +10,13 @@ open Spec.P256.Definitions
 open Lib.IntTypes
 
 open Spec.P256.Field
+open Spec.P256.Jacobian
 
 noextract
-val fromDomain_: a: int -> Tot (a: nat {a < prime})
+val fromDomain_: a: elem -> Tot elem
 
 noextract
-val fromDomainPoint: a: tuple3 nat nat nat -> Tot (r: tuple3 nat nat nat 
+val fromDomainPoint: a: pointJ -> Tot (r: pointJ
   {
     let x, y, z = a in
     let x3, y3, z3 = r in 
@@ -24,30 +25,30 @@ val fromDomainPoint: a: tuple3 nat nat nat -> Tot (r: tuple3 nat nat nat
 )
 
 noextract
-val toDomain_: a: int -> Tot nat
+val toDomain_: a: elem -> Tot elem
 
-val lemmaFromDomain: a: int -> Lemma (fromDomain_ (a) == a * modp_inv2 (pow2 256) % prime)
+val lemmaFromDomain: a: elem -> Lemma (fromDomain_ a == a * modp_inv2 (pow2 256) % prime)
 
-val lemmaToDomain: a: int -> Lemma (toDomain_(a) == a * (pow2 256) % prime)
+val lemmaToDomain: a: elem -> Lemma (toDomain_ a == a * (pow2 256) % prime)
 
-val lemmaToDomainAndBackIsTheSame: a: nat {a < prime} -> Lemma (fromDomain_ (toDomain_ a) == a)
+val lemmaToDomainAndBackIsTheSame: a: elem -> Lemma (fromDomain_ (toDomain_ a) == a)
   [SMTPat (fromDomain_ (toDomain_ a))]
 
-val lemmaFromDomainToDomain: a: nat { a < prime} -> Lemma (toDomain_ (fromDomain_ a) == a)
+val lemmaFromDomainToDomain: a: elem -> Lemma (toDomain_ (fromDomain_ a) == a)
 
-val lemmaFromDomainToDomainModuloPrime: a: int -> Lemma (a % prime == fromDomain_(toDomain_ a))
+val lemmaFromDomainToDomainModuloPrime: a: elem -> Lemma (a % prime == fromDomain_ (toDomain_ a))
 
-val inDomain_mod_is_not_mod: a: int -> Lemma (toDomain_ a == toDomain_ (a % prime))
+val inDomain_mod_is_not_mod: a: elem -> Lemma (toDomain_ a == toDomain_ (a % prime))
 
-val multiplicationInDomainNat: #k: nat -> #l: nat ->
+val multiplicationInDomainNat: #k: elem -> #l: elem ->
   a: nat {a == toDomain_ k /\ a < prime} -> 
   b: nat {b == toDomain_ l /\ b < prime} ->
   Lemma (
     let multResult = a * b * modp_inv2_prime (pow2 256) prime % prime in 
-    multResult == toDomain_ (k * l))
+    multResult == toDomain_ (k *% l))
 
-val additionInDomain: a: nat {a < prime} -> b: nat {b < prime} -> Lemma 
-  ((a + b) % prime == toDomain_ (fromDomain_ a + fromDomain_ b))
+val additionInDomain: a: elem -> b: elem -> 
+  Lemma (a +% b == toDomain_ (fromDomain_ a +% fromDomain_ b))
 
-val substractionInDomain: a: nat {a < prime} -> b: nat { b < prime} -> Lemma 
-  ((a - b) % prime == toDomain_ (fromDomain_ a - fromDomain_ b))
+val substractionInDomain: a: elem -> b: elem -> 
+  Lemma (a -% b == toDomain_ (fromDomain_ a -% fromDomain_ b))
